\documentclass[12pt,oneside,a4paper,fleqn]{article}
\usepackage{amsmath}
\usepackage{amssymb}
\usepackage[brazilian]{babel}
\usepackage[utf8]{inputenc}
\usepackage[T1]{fontenc}
\usepackage[margin=2cm]{geometry}
\usepackage[parfill]{parskip} % no indentation
\setlength{\parskip}{12pt} % redimensiona o tamanho do espaçamento entre parágrafos
\usepackage{multicol} % multiple columns per page
\begin{document}
\begin{multicols*}{2}
\begin{equation*}
\begin{cases}
5x+y+2z-2u+9v=-51 \\
-x-y+3z-u-v=4 \\
x-6y-10z+6u-9v=119 \\
x-2y-8z-2u-9v=121 \\
-9x-7y-6z-5u-6v=83
\end{cases}
\end{equation*}
\begin{equation*}
\text{Solução = }\left(5,-6,-3,-4,-8\right)
\end{equation*}
\vspace{\baselineskip}
\begin{equation*}
\begin{cases}
6x-6y-10z-7u-5v=-122 \\
-4x+7y+z-8u-8v=146 \\
6x+5y-3z+3u-4v=-17 \\
-2x-5y-4z+3u+4v=-66 \\
-10x-3y-7z+u+7v=-26
\end{cases}
\end{equation*}
\begin{equation*}
\text{Solução = }\left(-10,5,7,1,-9\right)
\end{equation*}
\vspace{\baselineskip}
\begin{equation*}
\begin{cases}
4x-8y+7z+5u+5v=141 \\
-9x-7y+4z+6u-10v=195 \\
-9x-y-3z-3u+5v=-92 \\
8x+7y-4z+9u+3v=-28 \\
-3x-4y+z+3u-2v=76
\end{cases}
\end{equation*}
\begin{equation*}
\text{Solução = }\left(2,-9,8,8,-7\right)
\end{equation*}
\vspace{\baselineskip}
\begin{equation*}
\begin{cases}
-6x+7y+5z+3u-3v=-88 \\
-9x+5y-7z-6u-6v=-133 \\
-9x+4y+3z-7u+3v=24 \\
-2x-5y+5z-7u-3v=92 \\
-10x-3y+6z+3u-4v=-11
\end{cases}
\end{equation*}
\begin{equation*}
\text{Solução = }\left(3,-9,7,-6,8\right)
\end{equation*}
\vspace{\baselineskip}
\begin{equation*}
\begin{cases}
-9x-9y+6z+7u+4v=94 \\
6x-10y+7z+9u-6v=-39 \\
-8x-9y-5z-7u+6v=183 \\
-6x+y-z-4u-2v=-4 \\
-5x-9y+9z-2u-9v=-68
\end{cases}
\end{equation*}
\begin{equation*}
\text{Solução = }\left(-3,-8,-8,1,9\right)
\end{equation*}
\vspace{\baselineskip}
\begin{equation*}
\begin{cases}
x-8y-7z+9u+7v=54 \\
-10x+9y-7z-3u+2v=-156 \\
-6x-3y+9z-5u-v=-11 \\
-10x-8y+z+4u+8v=-15 \\
-2x-3y-6z-5u-v=-28
\end{cases}
\end{equation*}
\begin{equation*}
\text{Solução = }\left(7,-6,3,3,-1\right)
\end{equation*}
\vspace{\baselineskip}
\begin{equation*}
\begin{cases}
3x+9y+4z-6u+5v=-84 \\
3x+4y-2z+4u-3v=-24 \\
3x-9y+5z+4u-v=-17 \\
5x+8y-10z-4u+9v=-50 \\
-10x-5y+7z+7u-9v=79
\end{cases}
\end{equation*}
\begin{equation*}
\text{Solução = }\left(-7,-4,-5,-3,-5\right)
\end{equation*}
\vspace{\baselineskip}
\begin{equation*}
\begin{cases}
3x+7y-7z+9u+9v=44 \\
-9x-6y-2z+7u-6v=15 \\
-7x+6y+9z+2u+8v=-95 \\
2x+6y-5z-7u-v=-36 \\
-3x+y-9z-7u-v=-62
\end{cases}
\end{equation*}
\begin{equation*}
\text{Solução = }\left(8,-2,-1,7,-4\right)
\end{equation*}
\vspace{\baselineskip}
\begin{equation*}
\begin{cases}
-6x-7y+6z+3u-3v=-145 \\
-x-5y-3z+u-5v=-18 \\
9x+8y-5z+8u-10v=-1 \\
5x-6y+3z-4u+v=4 \\
8x-3y-9z-5u-8v=128
\end{cases}
\end{equation*}
\begin{equation*}
\text{Solução = }\left(3,4,-10,-10,3\right)
\end{equation*}
\vspace{\baselineskip}
\begin{equation*}
\begin{cases}
2x+2y-z+9u+6v=-73 \\
7x+4y+8z-u-7v=-49 \\
-3x+7y+z-3u-6v=90 \\
-6x+4y-z-10u+2v=127 \\
8x+4y-3z-2u+8v=-41
\end{cases}
\end{equation*}
\begin{equation*}
\text{Solução = }\left(-8,5,-5,-6,-3\right)
\end{equation*}
\vspace{\baselineskip}
\begin{equation*}
\begin{cases}
-8x-6y-2z+u-10v=-47 \\
-3x+9y+8z-6u-3v=-93 \\
-9x-7y-3z+5u-9v=-49 \\
-x+7y-7z-10u-3v=70 \\
-10x+5y+5z-8u+v=-23
\end{cases}
\end{equation*}
\begin{equation*}
\text{Solução = }\left(1,-3,-9,-5,7\right)
\end{equation*}
\vspace{\baselineskip}
\begin{equation*}
\begin{cases}
-7x-3y-5z-u+7v=-49 \\
-6x+9y+7z-9u-7v=-86 \\
-5x+7y-10z+5u+7v=80 \\
-9x-5y-5z+u-8v=-1 \\
-x+y-5z+7u+6v=53
\end{cases}
\end{equation*}
\begin{equation*}
\text{Solução = }\left(7,4,-9,5,-4\right)
\end{equation*}
\vspace{\baselineskip}
\begin{equation*}
\begin{cases}
4x-2y+5z-7u-6v=27 \\
-4x-10y+5z-6u+7v=-3 \\
-4x-y-3z-2u+2v=25 \\
8x-3y-z+6u+v=-44 \\
9x-5y-10z+9u-7v=65
\end{cases}
\end{equation*}
\begin{equation*}
\text{Solução = }\left(-6,-5,-4,-1,-9\right)
\end{equation*}
\vspace{\baselineskip}
\begin{equation*}
\begin{cases}
8x-10y+6z-9u+3v=54 \\
-2x+5y+z+2u-2v=-15 \\
-3x-7y-3z-3u+6v=11 \\
-7x+5y+3z-u+3v=-24 \\
2x+8y-9z+5u+9v=-99
\end{cases}
\end{equation*}
\begin{equation*}
\text{Solução = }\left(-1,-2,-3,-9,-7\right)
\end{equation*}
\vspace{\baselineskip}
\begin{equation*}
\begin{cases}
-8x-5y+z+3u+4v=-31 \\
6x-10y+3z-9u-9v=107 \\
-2x+3y+9z-8u+4v=86 \\
-6x+7y-8z+8u-3v=-126 \\
5x-8y+8z-4u-3v=77
\end{cases}
\end{equation*}
\begin{equation*}
\text{Solução = }\left(3,-2,2,-9,2\right)
\end{equation*}
\vspace{\baselineskip}
\begin{equation*}
\begin{cases}
-5x-5y-9z+u+8v=-212 \\
5x+y-3z-5u-9v=116 \\
6x-10y-7z+9u+3v=-174 \\
-3x+2y+3z-2u+2v=19 \\
2x+4y-8z+6u+7v=-134
\end{cases}
\end{equation*}
\begin{equation*}
\text{Solução = }\left(6,6,9,-7,-8\right)
\end{equation*}
\vspace{\baselineskip}
\begin{equation*}
\begin{cases}
8x-8y+8z+5u-7v=237 \\
-10x+8y-3z+9u-10v=21 \\
-2x+8y+4z+2u+7v=-108 \\
4x-8y+z-2u-2v=92 \\
-7x+4y+7z+u+5v=-98
\end{cases}
\end{equation*}
\begin{equation*}
\text{Solução = }\left(7,-8,2,9,-8\right)
\end{equation*}
\vspace{\baselineskip}
\begin{equation*}
\begin{cases}
x+9y+8z+8u+6v=48 \\
-2x-10y-z-4u-v=-79 \\
-6x+6y+6z+6u+5v=73 \\
-3x+5y-4z+9u+8v=174 \\
-3x-5y+9z+6u-v=-93
\end{cases}
\end{equation*}
\begin{equation*}
\text{Solução = }\left(-6,8,-10,4,5\right)
\end{equation*}
\vspace{\baselineskip}
\begin{equation*}
\begin{cases}
5x+y-3z-7u+v=-62 \\
4x+6y-5z-5u-9v=-63 \\
8x+3y+5z-2u+9v=3 \\
-4x-y-9z+9u+4v=45 \\
3x-6y+8z-7u+5v=-29
\end{cases}
\end{equation*}
\begin{equation*}
\text{Solução = }\left(-3,2,3,6,2\right)
\end{equation*}
\vspace{\baselineskip}
\begin{equation*}
\begin{cases}
-6x+5y+8z+9u-6v=11 \\
6x-4y-7z-3u+4v=-42 \\
9x+6y-5z-3u-v=-85 \\
2x+3y+4z-9u+7v=39 \\
-4x-3y-2z+2u+9v=-7
\end{cases}
\end{equation*}
\begin{equation*}
\text{Solução = }\left(-5,-5,6,-6,-2\right)
\end{equation*}
\vspace{\baselineskip}
\begin{equation*}
\begin{cases}
-8x+y-6z+6u+9v=4 \\
-5x-10y-9z-4u-3v=145 \\
3x+7y+z+4u+6v=-75 \\
-4x+3y-5z-5u-2v=90 \\
-8x+2y-9z-u+6v=88
\end{cases}
\end{equation*}
\begin{equation*}
\text{Solução = }\left(-3,-2,-8,-8,-2\right)
\end{equation*}
\vspace{\baselineskip}
\begin{equation*}
\begin{cases}
8x-7y+z-9u-6v=-68 \\
7x+6y+8z-10u-4v=-38 \\
5x+8y-4z+4u+6v=4 \\
-9x+5y-8z-8u-5v=190 \\
-9x+y-7z-5u-2v=166
\end{cases}
\end{equation*}
\begin{equation*}
\text{Solução = }\left(-10,3,-6,-9,7\right)
\end{equation*}
\vspace{\baselineskip}
\begin{equation*}
\begin{cases}
-5x-2y-5z-7u+8v=-8 \\
-x-5y-10z-5u-5v=-18 \\
7x+y-4z-4u+7v=-72 \\
-2x+5y+7z-6u+4v=79 \\
-10x-3y-9z-10u-v=64
\end{cases}
\end{equation*}
\begin{equation*}
\text{Solução = }\left(-7,8,3,-4,-5\right)
\end{equation*}
\vspace{\baselineskip}
\begin{equation*}
\begin{cases}
-x+2y+8z+9u+2v=-98 \\
7x+y-2z-u+6v=11 \\
-2x-7y-10z-7u-2v=61 \\
-8x-4y-3z-3u-v=-18 \\
-2x+4y-2z+8u+v=-77
\end{cases}
\end{equation*}
\begin{equation*}
\text{Solução = }\left(6,1,-1,-8,-7\right)
\end{equation*}
\vspace{\baselineskip}
\begin{equation*}
\begin{cases}
3x+8y-4z-4u+7v=9 \\
-4x+2y-9z-6u-5v=12 \\
-2x-8y-3z+4u+3v=-2 \\
5x+3y+5z-2u-8v=-25 \\
7x+4y+4z+8u+6v=42
\end{cases}
\end{equation*}
\begin{equation*}
\text{Solução = }\left(-4,6,-3,8,-1\right)
\end{equation*}
\vspace{\baselineskip}
\begin{equation*}
\begin{cases}
-10x-6y+z-u-v=5 \\
-9x-9y+9z+5u-8v=-64 \\
-x-5y-3z-u+2v=2 \\
-4x-10y-10z-9u+6v=20 \\
-x+2y-4z-9u+4v=30
\end{cases}
\end{equation*}
\begin{equation*}
\text{Solução = }\left(-4,4,-2,2,7\right)
\end{equation*}
\vspace{\baselineskip}
\begin{equation*}
\begin{cases}
-2x-3y-7z+9u-v=-16 \\
-6x-3y-7z+4u-4v=38 \\
4x-3y-4z+7u+v=-34 \\
5x-7y+9z-5u+2v=74 \\
-7x+3y+7z-6u-9v=124
\end{cases}
\end{equation*}
\begin{equation*}
\text{Solução = }\left(-3,-8,4,-3,-9\right)
\end{equation*}
\vspace{\baselineskip}
\begin{equation*}
\begin{cases}
-x+8y-7z-3u+4v=-82 \\
-10x-10y-4z-5u+v=-34 \\
-6x-6y-5z+3u+7v=-86 \\
8x+2y+2z-7u+8v=27 \\
7x-9y+5z-8u+9v=71
\end{cases}
\end{equation*}
\begin{equation*}
\text{Solução = }\left(5,-3,6,-3,-5\right)
\end{equation*}
\vspace{\baselineskip}
\begin{equation*}
\begin{cases}
x-y+4z-6u-2v=33 \\
-4x+9y+z-u+v=-25 \\
-8x-4y-2z+9u+2v=-69 \\
x-3y-2z+7u+3v=-10 \\
3x-8y-10z+7u-5v=-54
\end{cases}
\end{equation*}
\begin{equation*}
\text{Solução = }\left(5,-2,2,-5,6\right)
\end{equation*}
\vspace{\baselineskip}
\begin{equation*}
\begin{cases}
2x-y-z-5u+8v=-20 \\
-9x-4y+3z-2u-5v=40 \\
-3x-5y-2z+3u+3v=66 \\
9x+y+5z+2u+6v=-71 \\
2x-9y+2z-8u+8v=-61
\end{cases}
\end{equation*}
\begin{equation*}
\text{Solução = }\left(-10,1,-4,7,4\right)
\end{equation*}
\vspace{\baselineskip}
\begin{equation*}
\begin{cases}
5x-y-6z-8u-8v=-42 \\
4x-10y-2z-4u-9v=3 \\
-2x+3y-7z-6u+3v=75 \\
2x-9y+9z+6u+8v=72 \\
-2x-4y+9z-6u-6v=9
\end{cases}
\end{equation*}
\begin{equation*}
\text{Solução = }\left(-9,-9,-3,-6,9\right)
\end{equation*}
\vspace{\baselineskip}
\begin{equation*}
\begin{cases}
8x+2y+3z-10u+v=-1 \\
-8x+3y-5z+5u+7v=-18 \\
-4x-y+z+7u-6v=0 \\
-4x-y-5z+6u+6v=-5 \\
x+9y+5z-4u-5v=-37
\end{cases}
\end{equation*}
\begin{equation*}
\text{Solução = }\left(-2,-6,5,-1,2\right)
\end{equation*}
\vspace{\baselineskip}
\begin{equation*}
\begin{cases}
9x-y-10z+3u-6v=-19 \\
-5x+4y+9z-8u+4v=64 \\
-10x+8y+8z-4u+3v=30 \\
-9x-4y+6z+7u+6v=-54 \\
-4x+8y-9z-6u-7v=-20
\end{cases}
\end{equation*}
\begin{equation*}
\text{Solução = }\left(6,5,2,-4,6\right)
\end{equation*}
\vspace{\baselineskip}
\begin{equation*}
\begin{cases}
4x-9y-9z+2u-4v=18 \\
-8x+8y-8z-9u-v=106 \\
7x-y-4z-10u+9v=-71 \\
2x+8y+3z+9u+8v=-10 \\
-3x+2y-z+7u-9v=79
\end{cases}
\end{equation*}
\begin{equation*}
\text{Solução = }\left(-5,4,-6,2,-4\right)
\end{equation*}
\vspace{\baselineskip}
\begin{equation*}
\begin{cases}
-2x+5y-4z-10u+6v=9 \\
3x-2y+2z+3u-5v=-4 \\
-10x+6y+5z+4u+8v=22 \\
6x-9y-9z+8u+2v=21 \\
3x+4y-4z-3u-6v=43
\end{cases}
\end{equation*}
\begin{equation*}
\text{Solução = }\left(4,9,-4,5,1\right)
\end{equation*}
\vspace{\baselineskip}
\begin{equation*}
\begin{cases}
-9x-3y-8z-10u+v=-162 \\
7x+6y-8z-4u-3v=30 \\
2x+2y+7z+5u+8v=1 \\
8x-5y-7z-8u-v=0 \\
3x+4y+5z+6u+9v=-12
\end{cases}
\end{equation*}
\begin{equation*}
\text{Solução = }\left(8,2,8,1,-10\right)
\end{equation*}
\vspace{\baselineskip}
\begin{equation*}
\begin{cases}
-4x-6y-4z+3u-4v=99 \\
-8x+6y+6z+9u-9v=-46 \\
-7x-3y-9z+5u-9v=94 \\
-6x+5y+2z-5u-5v=-118 \\
4x+7y+z-5u-3v=-158
\end{cases}
\end{equation*}
\begin{equation*}
\text{Solução = }\left(-4,-10,-6,9,7\right)
\end{equation*}
\vspace{\baselineskip}
\begin{equation*}
\begin{cases}
-8x+5y+8z-2u+2v=-100 \\
-2x-4y+4z-4u-7v=72 \\
-8x-8y+5z+9u+v=-64 \\
-8x+3y-9z+8u-2v=-145 \\
-x-y+2z-10u-2v=95
\end{cases}
\end{equation*}
\begin{equation*}
\text{Solução = }\left(7,-10,-1,-9,-2\right)
\end{equation*}
\vspace{\baselineskip}
\begin{equation*}
\begin{cases}
-x-7y-7z+3u-5v=-75 \\
-5x+4y-4z+6u+6v=2 \\
3x-4y+9z+3u+4v=-10 \\
8x+7y-5z+9u+8v=-93 \\
9x-5y-5z+7u+3v=-121
\end{cases}
\end{equation*}
\begin{equation*}
\text{Solução = }\left(-6,1,2,-10,6\right)
\end{equation*}
\vspace{\baselineskip}
\begin{equation*}
\begin{cases}
-5x+8y-2z-10u+7v=77 \\
5x+y+4z+7u-v=-31 \\
7x+y+4z+2u+2v=4 \\
-x+y+7z-3u-v=43 \\
7x-y+9z+u-2v=26
\end{cases}
\end{equation*}
\begin{equation*}
\text{Solução = }\left(2,4,2,-8,-3\right)
\end{equation*}
\vspace{\baselineskip}
\begin{equation*}
\begin{cases}
x-3y-2z+3u-3v=6 \\
-4x+y-4z-5u+2v=12 \\
-6x+8y+z+2u-v=117 \\
-x+y+8z-7u+v=-22 \\
8x+2y-8z+3u+8v=-97
\end{cases}
\end{equation*}
\begin{equation*}
\text{Solução = }\left(-8,7,-1,3,-8\right)
\end{equation*}
\vspace{\baselineskip}
\begin{equation*}
\begin{cases}
-4x+8y-z+8u+5v=-54 \\
-5x-7y-3z+6u-3v=105 \\
-x-5y-4z+2u-4v=85 \\
x-9y+9z-5u-2v=1 \\
-9x+2y-4z-6u-10v=9
\end{cases}
\end{equation*}
\begin{equation*}
\text{Solução = }\left(-1,-10,-9,1,1\right)
\end{equation*}
\vspace{\baselineskip}
\begin{equation*}
\begin{cases}
-4x-3y-5z+u-4v=61 \\
7x-6y+2z-4u-8v=68 \\
2x+3y-10z-2u+6v=-141 \\
-7x+9y-10z+6u-7v=-46 \\
-x+9y-8z-u+9v=-178
\end{cases}
\end{equation*}
\begin{equation*}
\text{Solução = }\left(-10,-9,6,-4,-7\right)
\end{equation*}
\vspace{\baselineskip}
\begin{equation*}
\begin{cases}
3x-3y+7z-9u+v=-110 \\
9x-8y-7z+5u-2v=-32 \\
-6x+2y+3z-5u+6v=45 \\
x-y+7z+9u-8v=-88 \\
7x+7y-9z+9u+2v=58
\end{cases}
\end{equation*}
\begin{equation*}
\text{Solução = }\left(-9,2,-9,2,4\right)
\end{equation*}
\vspace{\baselineskip}
\begin{equation*}
\begin{cases}
-x-2y+9z+3u+v=29 \\
-9x+4y+6z+8u+7v=-75 \\
8x+3y-z-4u+6v=-30 \\
-8x+8y+7z-2u-v=-78 \\
9x-y+8z+u-v=97
\end{cases}
\end{equation*}
\begin{equation*}
\text{Solução = }\left(7,-4,2,6,-8\right)
\end{equation*}
\vspace{\baselineskip}
\begin{equation*}
\begin{cases}
-9x+y-z-10u-9v=-158 \\
-4x-8y+5z+9u+4v=-3 \\
-x+8y+2z+u-4v=70 \\
9x-10y-2z-u-6v=-24 \\
2x+y+3z+7u+3v=96
\end{cases}
\end{equation*}
\begin{equation*}
\text{Solução = }\left(9,8,6,7,1\right)
\end{equation*}
\vspace{\baselineskip}
\begin{equation*}
\begin{cases}
-4x-9y-z-u+3v=103 \\
x-6y-z+4u+3v=44 \\
-8x+3y-6z+2u-2v=38 \\
2x+2y-z+3u-v=-29 \\
-9x-5y+6z-5u+4v=85
\end{cases}
\end{equation*}
\begin{equation*}
\text{Solução = }\left(-6,-8,-3,-1,1\right)
\end{equation*}
\vspace{\baselineskip}
\begin{equation*}
\begin{cases}
2x-7y+4z-5u+5v=-2 \\
-4x-4y-3z-2u-9v=46 \\
-2x-5y-8z+6u-8v=76 \\
2x+2y+z+2u+9v=-6 \\
2x+7y-7z+u-6v=2
\end{cases}
\end{equation*}
\begin{equation*}
\text{Solução = }\left(-7,-4,-9,-1,3\right)
\end{equation*}
\vspace{\baselineskip}
\begin{equation*}
\begin{cases}
-3x-10y-8z-9u-7v=90 \\
9x+9y+6z-u+3v=-83 \\
-2x+2y-10z+7u-9v=15 \\
3x-y-8z-5u+5v=95 \\
x-8y-9z+5u+6v=85
\end{cases}
\end{equation*}
\begin{equation*}
\text{Solução = }\left(-5,-1,-8,-4,5\right)
\end{equation*}
\vspace{\baselineskip}
\begin{equation*}
\begin{cases}
7x+5y+8z+5u+6v=148 \\
6x-10y-z-6u-3v=-5 \\
-6x-3y-10z-9u-9v=-130 \\
-8x+6y-7z+2u+8v=-37 \\
-4x-7y+9z-8u+5v=68
\end{cases}
\end{equation*}
\begin{equation*}
\text{Solução = }\left(8,7,7,-7,6\right)
\end{equation*}
\vspace{\baselineskip}
\begin{equation*}
\begin{cases}
-x-3y+6z+9u-5v=-23 \\
-4x+3y+z+5u-2v=-14 \\
7x-5y-8z-8u+v=-3 \\
9x-7y+9z+5u+6v=-34 \\
-10x+9y-7z-u-8v=44
\end{cases}
\end{equation*}
\begin{equation*}
\text{Solução = }\left(6,9,7,-8,-8\right)
\end{equation*}
\vspace{\baselineskip}
\begin{equation*}
\begin{cases}
8x-y+2z-7u-v=-14 \\
-7x-6y+7z+5u+5v=-3 \\
7x+9y-3z-4u-7v=-26 \\
-7x+8y-4z-2u-v=82 \\
3x+6y+3z+7u+2v=-116
\end{cases}
\end{equation*}
\begin{equation*}
\text{Solução = }\left(-9,-2,-4,-9,-1\right)
\end{equation*}
\vspace{\baselineskip}
\begin{equation*}
\begin{cases}
5x+6y-2z-3u-4v=82 \\
7x+3y+4z+2u-8v=51 \\
6x+9y-8z-9u-3v=132 \\
-3x+7y+3z+u-6v=21 \\
-2x-y+5z+9u-5v=-26
\end{cases}
\end{equation*}
\begin{equation*}
\text{Solução = }\left(6,7,-6,2,-1\right)
\end{equation*}
\vspace{\baselineskip}
\begin{equation*}
\begin{cases}
3x-2y-5z+4u+2v=-105 \\
-5x-7y+7z+7u-3v=109 \\
-9x+9y+4z+3u-6v=60 \\
4x+9y+7z-2u-8v=74 \\
-5x-8y-6z-8u+v=94
\end{cases}
\end{equation*}
\begin{equation*}
\text{Solução = }\left(-6,-7,9,-9,-10\right)
\end{equation*}
\vspace{\baselineskip}
\begin{equation*}
\begin{cases}
-8x-10y-10z+7u+5v=-181 \\
4x+3y+2z+9u+3v=0 \\
x+3y-4z+9u-4v=-66 \\
-7x-2y+8z+2u-2v=-5 \\
9x-4y-3z+3u-10v=-67
\end{cases}
\end{equation*}
\begin{equation*}
\text{Solução = }\left(3,7,6,-6,3\right)
\end{equation*}
\vspace{\baselineskip}
\begin{equation*}
\begin{cases}
2x-3y-8z-4u+6v=16 \\
6x-7y-5z+8u-2v=50 \\
3x-4y+3z+7u+7v=6 \\
-5x-y+8z+3u+3v=26 \\
-10x+2y+7z-u-v=37
\end{cases}
\end{equation*}
\begin{equation*}
\text{Solução = }\left(-7,-10,-2,1,-2\right)
\end{equation*}
\vspace{\baselineskip}
\begin{equation*}
\begin{cases}
-7x-9y+5z-10u+7v=-165 \\
4x+y+z-4u-3v=78 \\
7x-7y+3z-5u-6v=65 \\
3x-8y-2z+3u-7v=7 \\
6x-y-z+7u-8v=96
\end{cases}
\end{equation*}
\begin{equation*}
\text{Solução = }\left(7,9,3,-2,-10\right)
\end{equation*}
\vspace{\baselineskip}
\begin{equation*}
\begin{cases}
8x-5y+9z+9u+9v=208 \\
-10x-4y+5z-2u+v=8 \\
3x+3y-5z-6u+8v=-7 \\
4x-5y-z+3u+4v=41 \\
4x-4y+z-10u-8v=-89
\end{cases}
\end{equation*}
\begin{equation*}
\text{Solução = }\left(3,1,9,5,7\right)
\end{equation*}
\vspace{\baselineskip}
\begin{equation*}
\begin{cases}
7x-9y-z+5u+5v=-109 \\
-8x+7y+8z-7u+5v=58 \\
-7x+9y+2z+6u+8v=-9 \\
4x-3y+5z-5u+v=-6 \\
-8x+8y+3z-5u-7v=90
\end{cases}
\end{equation*}
\begin{equation*}
\text{Solução = }\left(1,8,-6,-9,-1\right)
\end{equation*}
\vspace{\baselineskip}
\begin{equation*}
\begin{cases}
-6x-5y-4z+9u+v=-81 \\
-10x+9y-10z+4u-6v=-23 \\
-2x-5y+2z+5u-9v=-89 \\
-10x-7y+5z-8u+5v=-25 \\
-3x-9y+z-6u-6v=-106
\end{cases}
\end{equation*}
\begin{equation*}
\text{Solução = }\left(2,9,5,-1,5\right)
\end{equation*}
\vspace{\baselineskip}
\end{multicols*}
\end{document}
